Expr.v
@@ -12,37 +12,47 @@ Inductive exp : Type :=
 | Sort : nat -> exp
 | Free : name -> exp
 
-| Pi : exp -> {bind exp} -> exp
+| Pi : exp -> {bind 1 of exp} -> exp
 (* | Lam : exp -> {bind exp} -> exp *)
-| Lam : {bind exp} -> exp
+| Lam : {bind 1 of exp} -> exp
 | App  : exp -> exp -> exp
 
 | Sigma : exp -> {bind exp} -> exp
-| S_mk : exp ->  exp -> exp
-| S_rec : {bind 2 of exp} -> exp -> exp
-(* | S_p1 : exp -> exp *)
-(* | S_p2 : exp -> exp *)
+| Pair__sigma : exp ->  exp -> exp
+| Rec__sigma : {bind 2 of exp} -> exp -> exp
 
-| Sum : exp -> exp -> exp
-| Sum_inl : exp -> exp
-| Sum_inr : exp -> exp
-| Split : {bind exp} -> {bind exp} -> exp -> exp
-
-| Unit : exp
-| unit : exp
-
+| Path : exp -> exp -> exp
+| Rec__path : exp -> exp -> exp
+| Refl__path : exp -> exp
+ 
 (* | Empty :  exp *)
 (* | empty_rec : exp -> exp *)
 
-| Mu : desc -> exp
-(* | Wrap : exp -> exp *)
-(* | Unwrap : exp -> exp *)
-| mu : desc -> {bind 2 of exp} -> exp -> exp.
+| Desc : exp
+| Ind__desc : exp
+| Sum__desc : exp -> exp -> exp
+| Prd__desc : exp -> exp -> exp
+| Unit__desc : exp
+| Fix__desc : exp -> exp
+| Rec__desc : exp
+            -> {bind 4 of exp} -> {bind 4 of exp}
+            -> exp
+            -> {bind 2 of exp}
+            -> exp -> exp
 
-Instance Ids_exp : Ids exp. derive. Defined.
-Instance Rename_exp : Rename exp. derive. Defined.
-Instance Subst_exp : Subst exp. derive. Defined.
-Instance SubstLemmas_exp : SubstLemmas exp. derive. Qed.
+| Mu : exp -> exp -> exp
+| Wrap__mu : exp -> exp
+| Inl__mu : exp -> exp
+| Inr__mu : exp -> exp
+| Pair__mu : exp -> exp -> exp
+| Unit__mu : exp
+| Fix__mu : exp -> exp
+| Rec__mu : {bind 2 of exp}
+          -> {bind 2 of exp} -> {bind 2 of exp}
+          -> {bind 4 of exp}
+          -> exp
+          -> {bind 2 of exp}
+          -> exp -> exp.
 
 Hint Resolve internal_nat_dec_lb internal_nat_dec_bl.
 
@@ -51,8 +61,9 @@ Hint Resolve exp_dec_lb.
 
 Hint Extern 1 => match goal with [H: (_ && _)        |- _] => apply andb_prop in H; destruct H end.
 Hint Extern 1 => match goal with [H: (_ && _) = true |- _] => apply andb_prop in H; destruct H end.
-Lemma exp_dec_bl : forall x y, exp_beq x y -> x = y. unfold is_true; induction x; destruct y; 
-                                               simpl; intros; f_equal; congruence || auto. Qed.
+
+Lemma exp_dec_bl : forall x y, exp_beq x y -> x = y. unfold is_true; induction x; destruct y; simpl; intros; 
+                                               discriminate || f_equal; destr bands; auto. Qed.
 Hint Resolve exp_dec_bl.  
 
 Lemma exp_eqnP : Equality.axiom exp_beq.
@@ -61,46 +72,45 @@ Proof. intros x y; apply (iffP idP); auto. Qed.
 Canonical exp_eqMixin := EqMixin exp_eqnP.
 Canonical exp_eqType := EqType exp exp_eqMixin.
 
+Instance Ids_exp : Ids exp. derive. Defined.
+Instance Rename_exp : Rename exp. derive. Defined.
+Instance Subst_exp : Subst exp. derive. Defined.
+Instance SubstLemmas_exp : SubstLemmas exp. derive. Qed.
+
+Tactic Notation "arewrite" := autorewrite with autosubst.
+
 Infix ":>>" := Pi (at level 20, right associativity).
 Infix ":#>" := Lam (at level 30, right associativity).
 Infix ":$:" := App (at level 50, left associativity).
-Notation "<< a ;; b >>" := (S_mk a b).
+Notation "<< a ;; b >>" := (Pair__sigma a b).
 
-Notation Prd A B := (Sigma A (B.[ren (+1)])).
-Infix ":*:" := Prd (at level 10).
-
-Fixpoint D_efunc (D : desc) (X : exp) : exp :=
-  match D with
-      d_One => Unit
-    | d_Sum A B => Sum (D_efunc A X) (D_efunc B X)
-    | d_Prd A B => Prd (D_efunc A X) (D_efunc B X)
-    | d_Ind => X
-  end.
+(* Notation Prd A B := (Sigma A (B.[ren (+1)])). *)
+(* Infix ":*:" := Prd (at level 10). *)
 
 Notation wk n := (ren (+ n)).
 
-Notation S_p1 e := (S_rec (Bind 1) e).
-Notation S_p2 e := (S_rec (Bind 0) e).
+Notation S_p1 e := (Rec__sigma (Bind 1) e).
+Notation S_p2 e := (Rec__sigma (Bind 0) e).
 
-Fixpoint All (d : desc) (P : {bind exp}) (e : exp) :=
-  match d with 
-      d_One => Unit
-    | d_Ind => P.[e/]
-    | d_Sum d1 d2 => Split
-                      (All d1 P.[up (wk 1)] (Bind 0))
-                      (All d2 P.[up (wk 1)] (Bind 0))
-                      e
-    | d_Prd d1 d2 => S_rec (Prd (All d1 P.[up (wk 2)] (Bind 1)) (All d2 P.[up (wk 2)] (Bind 0))) e
-  end.
+(* Fixpoint All (d : desc) (P : {bind exp}) (e : exp) := *)
+(*   match d with  *)
+(*       d_One => Unit *)
+(*     | d_Ind => P.[e/] *)
+(*     | d_Sum d1 d2 => Split *)
+(*                       (All d1 P.[up (wk 1)] (Bind 0)) *)
+(*                       (All d2 P.[up (wk 1)] (Bind 0)) *)
+(*                       e *)
+(*     | d_Prd d1 d2 => S_rec (Prd (All d1 P.[up (wk 2)] (Bind 1)) (All d2 P.[up (wk 2)] (Bind 0))) e *)
+(*   end. *)
 
-Fixpoint rall (d : desc) (r : {bind exp}) (e : exp) :=
-  match d with
-      d_One => unit
-    | d_Ind => r.[e/]
-    | d_Sum d1 d2 => Split
-                      (* (All (d_Sum d1 d2) P (Bind 0))  *)
-                      (rall d1 r.[up (wk 1)] (Bind 0))
-                      (rall d2 r.[up (wk 1)] (Bind 0))
-                      e
-    | d_Prd d1 d2 => S_rec (S_mk (rall d1 r.[up (wk 2)] (Bind 1)) (rall d2 r.[up (wk 2)] (Bind 0))) e
-  end.
+(* Fixpoint rall (d : desc) (r : {bind exp}) (e : exp) := *)
+(*   match d with *)
+(*       d_One => unit *)
+(*     | d_Ind => r.[e/] *)
+(*     | d_Sum d1 d2 => Split *)
+(*                       (* (All (d_Sum d1 d2) P (Bind 0))  *) *)
+(*                       (rall d1 r.[up (wk 1)] (Bind 0)) *)
+(*                       (rall d2 r.[up (wk 1)] (Bind 0)) *)
+(*                       e *)
+(*     | d_Prd d1 d2 => S_rec (S_mk (rall d1 r.[up (wk 2)] (Bind 1)) (rall d2 r.[up (wk 2)] (Bind 0))) e *)
+(*   end. *)
