Reduction.v
@@ -2,28 +2,6 @@ Require Import Prelude.
 Require Import Expr.
 Require Import Scoping.
 
-(* Fixpoint canonize e := *)
-(*   match e with *)
-(*     | Wrap (Unwrap e') => canonize e' *)
-(*     | Unwrap (Wrap e') => canonize e' *)
-(*     | Lam b => Lam (canonize b) *)
-(*     | A :>> B => canonize A :>> canonize B *)
-(*     | f :$: x => canonize f :$: canonize x *)
-(*     | Sigma A B => Sigma (canonize A) (canonize B) *)
-(*     | S_mk a b => S_mk (canonize a) (canonize b) *)
-(*     | S_p1 a => S_p1 (canonize a)  *)
-(*     | S_p2 b => S_p2 (canonize b) *)
-(*     | Sum A B => Sum (canonize A) (canonize B) *)
-(*     | Sum_inl a => Sum_inl (canonize a) *)
-(*     | Sum_inr b => Sum_inr (canonize b) *)
-(*     | Split a b ab => Split (canonize a) (canonize b) (canonize ab) *)
-(*     | empty_rec e => empty_rec (canonize e) *)
-(*     (* | Wrap e => Wrap (canonize e) *) *)
-(*     (* | Unwrap e => Unwrap (canonize e) *) *)
-(*     | mu D r d => mu D (canonize r) (canonize d) *)
-(*     | _ => e *)
-(*   end. *)
- 
 Notation env a := (Expr.name -> option a).
 Reserved Notation "a ::> b" (at level 50).
 Variable const_vals : env exp.
@@ -42,41 +20,83 @@ Inductive par_step : relation exp :=
 | P_beta   : forall u f b a a', f ::> Lam b -> a ::> a' -> u = b.[a'/] -> (f :$: a) ::> u
  
 | P_sig    : forall A A' B B', A ::> A' -> B ::> B' -> Sigma A B ::> Sigma A' B'
-| P_smk    : forall a a' b b', a ::> a' -> b ::> b' -> S_mk a b ::> S_mk a' b'
-| P_srec   : forall r r' p p', r ::> r' -> p ::> p' -> S_rec r p ::> S_rec r' p'
-| P_srec_beta : forall u r r' p a b, r ::> r' -> p ::> S_mk a b -> u = r'.[b,a/] -> S_rec r p ::> u
-(* | P_pi1    : forall s s', s ::> s' -> S_p1 s ::> S_p1 s' *)
-(* | P_pi2    : forall s s', s ::> s' -> S_p2 s ::> S_p2 s' *)
-(* | P_p1beta : forall s a b, s ::> S_mk a b -> S_p1 s ::> a *)
-(* | P_p2beta : forall s a b, s ::> S_mk a b -> S_p2 s ::> b *)
- 
-| P_Sum    : forall A A' B B', A ::> A' -> B ::> B' -> Sum A B ::> Sum A' B'
-| P_inl    : forall a a', a ::> a' -> Sum_inl a ::> Sum_inl a'
-| P_inr    : forall b b', b ::> b' -> Sum_inr b ::> Sum_inr b'
-(* | P_split  : forall C C' a a' b b' ab ab', C ::> C' -> a ::> a' -> b ::> b' -> ab ::> ab' -> Split C a b ab ::> Split C' a' b' ab' *)
-| P_split  : forall a a' b b' ab ab',  a ::> a' -> b ::> b' -> ab ::> ab' -> Split a b ab ::> Split a' b' ab'
-| P_split_l : forall u ca ca' cb ab a, ca ::> ca' -> ab ::> Sum_inl a -> u = ca'.[a/] -> Split ca cb ab ::> u
-| P_split_r : forall u ca cb cb' ab b, cb ::> cb' -> ab ::> Sum_inr b -> u = cb'.[b/] -> Split ca cb ab ::> u
- 
-(* | P_emrec  : forall C C' e e', C ::> C' -> e ::> e' -> empty_rec C e ::> empty_rec C' e' *)
-(* | P_emrec  : forall e e', e ::> e' -> empty_rec e ::> empty_rec e' *)
- 
-(* | P_wrap   : forall m m', m ::> m' -> Wrap m ::> Wrap m' *)
-(* | P_unwrap : forall m m', m ::> m' -> Unwrap m ::> Unwrap m' *)
+| P_smk    : forall a a' b b', a ::> a' -> b ::> b' -> Pair__sigma a b ::> Pair__sigma a' b'
+| P_srec   : forall r r' p p', r ::> r' -> p ::> p' -> Rec__sigma r p ::> Rec__sigma r' p'
+| P_srec_beta : forall u r r' p a b, r ::> r' -> p ::> Pair__sigma a b -> u = r'.[b,a/] -> Rec__sigma r p ::> u
 
-(* | P_wrap_unwrap : forall m m', m ::> Unwrap m' -> Wrap m ::> m' *)
-(* | P_unwrap_wrap : forall m m', m ::> Wrap m' -> Unwrap m ::> m' *)
-(* | P_wrap_unwrap_eta : forall m m', m ::> Wrap (Unwrap m') -> m ::> m' *)
-(* | P_unwrap_wrap_eta : forall m m', m ::> Unwrap (Wrap m') -> m ::> m' *)
-                                                     
-(* | P_Mu : forall D, Mu D ::> D_efunc D (Mu D) *)
-| P_mu : forall D r r' d d', r ::> r' -> d ::> d' -> mu D r d ::> mu D r' d'
-| P_mu_rec : forall u D r r' e e', r ::> r' -> e ::> e' -> 
-                              u = r'.[rall D (mu D r'.[upn 2 (wk 1)] (Bind 0)) e', e'/] ->
-                              (* u = (r' :$: e' :$: rall D (mu D r'.[wk 1] (Bind 0)) e') -> *)
-                              mu D r e ::> u
-(* | P_mu_rec : forall D P P' r r' e e', P ::> P' -> r ::> r' -> e ::> Wrap e' ->  *)
-                                 (* mu D P r e ::> (r' :$: Wrap e' :$: rall P D (mu D P.[wk 1] r.[wk 1] (Bind 0)) e) *)
+| P_path : forall x x' y y',  x ::> x' -> y ::> y' -> Path x y ::> Path x' y'
+| P_refl : forall x x', x ::> x' -> Refl__path x ::> Refl__path x'
+| P_prec : forall c c' p p', c ::> c' -> p ::> p' -> Rec__path c p ::> Rec__path c' p'
+| P_precr : forall c c' p x, c ::> c' -> p ::> Refl__path x -> Rec__path c p ::> c'
+
+| P_sdesc : forall A A' B B', A ::> A' -> B ::> B' -> Sum__desc A B ::> Sum__desc A' B'
+| P_pdesc : forall A A' B B', A ::> A' -> B ::> B' -> Prd__desc A B ::> Prd__desc A' B'
+| P_fdesc : forall D D', D ::> D' -> Fix__desc D ::> Fix__desc D'
+| P_descr : forall i i' s s' p p' u u' f f' d d',
+              i ::> i' -> s ::> s' -> p ::> p' -> u ::> u' -> f ::> f' -> d ::> d' ->
+              Rec__desc i s p u f d ::> Rec__desc i' s' p' u' f' d'
+
+| P_descr_i : forall i i' s p u f d, i ::> i' -> d ::> Ind__desc -> Rec__desc i s p u f d ::> i'
+| P_descr_s : forall i i' s s' p p' u u' f f' d A B e,
+                i ::> i' -> s ::> s' -> p ::> p' -> u ::> u' -> f ::> f' ->
+                d ::> Sum__desc A B ->
+                e = s'.[Rec__desc i' s' p' u' f' B, B, Rec__desc i' s' p' u' f' A, A/] ->
+                Rec__desc i s p u f d ::> e
+| P_descr_p : forall i i' s s' p p' u u' f f' d A B e,
+                i ::> i' -> s ::> s' -> p ::> p' -> u ::> u' -> f ::> f' ->
+                d ::> Prd__desc A B ->
+                e = p'.[Rec__desc i' s' p' u' f' B, B, Rec__desc i' s' p' u' f' A, A/] ->
+                Rec__desc i s p u f d ::> e
+| P_descr_u : forall i s p u u' f d,
+                u ::> u' -> d ::> Unit__desc ->
+                Rec__desc i s p u f d ::> u'
+| P_descr_f : forall i i' s s' p p' u u' f f' d D e,
+                i ::> i' -> s ::> s' -> p ::> p' -> u ::> u' -> f ::> f' ->
+                d ::> Fix__desc D ->
+                e = f'.[Rec__desc i' s' p' u' f' D,D/] ->
+                Rec__desc i s p u f d ::> e
+
+| P_mu : forall D1 D1' D2 D2', D1 ::> D1' -> D2 ::> D2' -> Mu D1 D2 ::> Mu D1' D2'
+| P_wmu : forall m m', m ::> m' -> Wrap__mu m ::> Wrap__mu m'
+| P_inlmu : forall a a', a ::> a' -> Inl__mu a ::> Inl__mu a'
+| P_inrmu : forall b b', b ::> b' -> Inr__mu b ::> Inr__mu b'
+| P_parmu : forall a a' b b', a ::> a' -> b ::> b' -> Pair__mu a b ::> Pair__mu a' b'
+| P_fixmu : forall f f', f ::> f' -> Fix__mu f ::> Fix__mu f'
+| P_murec : forall w w' il il' ir ir' p p' u u' f f' m m',
+              w ::> w' -> il ::> il' -> ir ::> ir' -> p ::> p' -> u ::> u' -> f ::> f' ->
+              m ::> m' ->
+              Rec__mu w il ir p u f m ::> Rec__mu w' il' ir' p' u' f' m'
+ 
+| P_murecw : forall w w' il il' ir ir' p p' f f' u u' m m' e,
+              w ::> w' -> il ::> il' -> ir ::> ir' -> p ::> p' -> u ::> u' -> f ::> f' ->
+              m ::> Wrap__mu m' ->
+              e = w'.[Rec__mu w' il' ir' p' u' f' m',m'/] ->
+              Rec__mu w il ir p u f m ::> e
+| P_murecl : forall w w' il il' ir ir' p p' u u' f f' m l e,
+              w ::> w' -> il ::> il' -> ir ::> ir' -> p ::> p' -> u ::> u' -> f ::> f' ->
+              m ::> Inl__mu l ->
+              e = il'.[Rec__mu w' il' ir' p' u' f' l,l/] ->
+              Rec__mu w il ir p u f m ::> e
+| P_murecr : forall w w' il il' ir ir' p p' u u' f f' m r e,
+              w ::> w' -> il ::> il' -> ir ::> ir' -> p ::> p' -> u ::> u' -> f ::> f' ->
+              m ::> Inr__mu r ->
+              e = ir'.[Rec__mu w' il' ir' p' u' f' r,r/] ->
+              Rec__mu w il ir p u f m ::> e
+| P_murecp : forall w w' il il' ir ir' p p' u u' f f' m a b e,
+              w ::> w' -> il ::> il' -> ir ::> ir' -> p ::> p' -> u ::> u' -> f ::> f' ->
+              m ::> Pair__mu a b ->
+              e = p'.[Rec__mu w' il' ir' p' u' f' b, b, Rec__mu w' il' ir' p' u' f' a, a/] ->
+              Rec__mu w il ir p u f m ::> e
+| P_murecu : forall w il ir p u u' f m,
+               u ::> u' -> m ::> Unit__mu ->
+               Rec__mu w il ir p u f m ::> u'
+              
+| P_murecf : forall w w' il il' ir ir' p p' u u' f f' m M e,
+              w ::> w' -> il ::> il' -> ir ::> ir' -> p ::> p' -> u ::> u' -> f ::> f' ->
+              m ::> Fix__mu M ->
+              e = f'.[Rec__mu w' il' ir' p' u' f' M,M/] ->
+              Rec__mu w il ir p u f m ::> e
+
 where "a ::> b" := (par_step a b).
 
 Hypothesis consts_closed : forall nm e, const_vals nm = Some e -> closed e.
@@ -92,37 +112,53 @@ Fixpoint rho (e : exp) : exp :=
                   end
 
     | Sigma A B => Sigma (rho A) (rho B)
-    | S_mk a b => S_mk (rho a) (rho b)
-    | S_rec r ab => match rho ab with
-                     | S_mk a b => (rho r).[b,a/]
-                     | ab' => S_rec (rho r) ab'
-                   end
+    | Pair__sigma a b => Pair__sigma (rho a) (rho b)
+    | Rec__sigma r ab => match rho ab with
+                        | Pair__sigma a b => (rho r).[b,a/]
+                        | ab' => Rec__sigma (rho r) ab'
+                      end
 
-    | Sum A B => Sum (rho A) (rho B)
-    | Sum_inl a => Sum_inl (rho a)
-    | Sum_inr b => Sum_inr (rho b)
-    | Split ca cb ab => match rho ab with
-                         | Sum_inl a => (rho ca).[a/]
-                         | Sum_inr b => (rho cb).[b/]
-                         | ab' => Split (rho ca) (rho cb) ab'
-                       end
+    | Path x y => Path (rho x) (rho y)
+    | Refl__path x => Refl__path (rho x)
+    | Rec__path c p => match rho p with
+                      | Refl__path x => (rho c)
+                      | p' => Rec__path (rho c) p'
+                    end
+    
+    | Sum__desc A B => Sum__desc (rho A) (rho B)
+    | Prd__desc A B => Prd__desc (rho A) (rho B)
+    | Fix__desc D => Fix__desc (rho D)
 
-    (* | empty_rec e => empty_rec (rho e) *)
+    | Rec__desc i s p u f d => 
+      let i := rho i in let s := rho s in let p := rho p in let u := rho u in let f := rho f in let d := rho d in
+      match d with
+        | Ind__desc => i
+        | Sum__desc A B => s.[Rec__desc i s p u f B, B, Rec__desc i s p u f A, A/]
+        | Prd__desc A B => p.[Rec__desc i s p u f B, B, Rec__desc i s p u f A, A/]
+        | Fix__desc D => f.[Rec__desc i s p u f D, D/]
+        | Unit__desc => u
+        | _ => Rec__desc i s p u f d
+      end
+                             
+    | Mu D1 D2 => Mu (rho D1) (rho D2)
+    | Wrap__mu m => Wrap__mu (rho m)
+    | Inl__mu a => Inl__mu (rho a)
+    | Inr__mu b => Inr__mu (rho b)
+    | Pair__mu a b => Pair__mu (rho a) (rho b)
+    | Fix__mu m => Fix__mu (rho m)
 
-    (* | Wrap m => Wrap (rho m) *)
-    (* | Wrap m => match rho m with *)
-    (*              | Unwrap m' => m' *)
-    (*              | m' => Wrap m' *)
-    (*            end *)
-
-    (* | Unwrap m => Unwrap (rho m) *)
-    (* | Unwrap m => match rho m with *)
-    (*                | Wrap m' => m' *)
-    (*                | m' => Unwrap m' *)
-    (*              end *)
-
-    (* | Mu D => D_efunc D (Mu D) *)
-    | mu D r d => (rho r).[rall D (mu D (rho r).[upn 2 (wk 1)] (Bind 0)) (rho d), (rho d)/]
+    | Rec__mu w il ir p u f m => 
+      let w := rho w in let il := rho il in let ir := rho ir in let p := rho p in 
+      let u := rho u in let f := rho f in let m := rho m in
+      match m with
+        | Wrap__mu m => w.[Rec__mu w il ir p u f m,m/]
+        | Inl__mu l => il.[Rec__mu w il ir p u f l,l/]
+        | Inr__mu r => ir.[Rec__mu w il ir p u f r,r/]
+        | Pair__mu a b => p.[Rec__mu w il ir p u f b, b, Rec__mu w il ir p u f a, a/]
+        | Unit__mu => u
+        | Fix__mu d => f.[Rec__mu w il ir p u f d, d/]
+        | _ => Rec__mu w il ir p u f m
+      end
 
     | _ => e
   end.
@@ -136,20 +172,57 @@ Proof. induction e; simpl; try solve[try destruct match;eauto].
 Qed.
 Hint Resolve rho_eval_to.
 
-Tactic Notation "invert" "value" "steps" :=
+Tactic Notation "econstructor" "beta" :=
+  match goal with
+    | [H: context[_ ::> Lam _]         |- App _ _ ::> _] => eapply P_beta
+    | [H: context[_ ::> Pair__sigma _ _] |- Rec__sigma _ _ ::> _] => eapply P_srec_beta
+    | [H: context[_ ::> Refl__path _]    |- Rec__path _ _ ::> _] => eapply P_precr
+
+    | [H: context[_ ::> Ind__desc]       |- Rec__desc _ _ _ _ _ _ ::> _] => eapply P_descr_i
+    | [H: context[_ ::> Sum__desc _ _]   |- Rec__desc _ _ _ _ _ _ ::> _] => eapply P_descr_s
+    | [H: context[_ ::> Prd__desc _ _]   |- Rec__desc _ _ _ _ _ _ ::> _] => eapply P_descr_p
+    | [H: context[_ ::> Unit__desc]      |- Rec__desc _ _ _ _ _ _ ::> _] => eapply P_descr_u
+    | [H: context[_ ::> Fix__desc _]     |- Rec__desc _ _ _ _ _ _ ::> _] => eapply P_descr_f
+
+    | [H: context[_ ::> Wrap__mu _]      |- Rec__mu _ _ _ _ _ _ _ ::> _] => eapply P_murecw
+    | [H: context[_ ::> Inl__mu _]       |- Rec__mu _ _ _ _ _ _ _ ::> _] => eapply P_murecl
+    | [H: context[_ ::> Inr__mu _]       |- Rec__mu _ _ _ _ _ _ _ ::> _] => eapply P_murecr
+    | [H: context[_ ::> Pair__mu _ _]    |- Rec__mu _ _ _ _ _ _ _ ::> _] => eapply P_murecp
+    | [H: context[_ ::> Unit__mu]        |- Rec__mu _ _ _ _ _ _ _ ::> _] => eapply P_murecu
+    | [H: context[_ ::> Fix__mu _]       |- Rec__mu _ _ _ _ _ _ _ ::> _] => eapply P_murecf
+  end.
+
+Tactic Notation "econstructor" "par" :=
+  eapply P_ref + eapply P_free +
+  eapply P_pi + eapply P_lam + eapply P_app +
+  eapply P_sig + eapply P_smk + eapply P_srec +
+  eapply P_path + eapply P_refl + eapply P_prec +
+  eapply P_sdesc + eapply P_pdesc + eapply P_fdesc + eapply P_descr +
+  eapply P_mu + eapply P_wmu + eapply P_inlmu + eapply P_inrmu + eapply P_parmu + eapply P_fixmu + eapply P_murec.
+
+Tactic Notation "econstructor" "step" := econstructor beta + econstructor par.
+
+Tactic Notation "invert" "value" "step" :=
   match goal with
     | [H: Bind _ ::> _ |- _] => inverts H
     | [H: Sort _ ::> _ |- _] => inverts H
     | [H: Pi _ _ ::> _ |- _] => inverts H
     | [H: Lam _ ::> _ |- _] => inverts H
     | [H: Sigma _ _ ::> _ |- _] => inverts H
-    | [H: S_mk _ _ ::> _ |- _] => inverts H
-    | [H: Sum _ _ ::> _ |- _] => inverts H
-    | [H: Sum_inl _ ::> _ |- _] => inverts H
-    | [H: Sum_inr _ ::> _ |- _] => inverts H
-    | [H: Unit ::> _ |- _] => inverts H
-    | [H: unit ::> _ |- _] => inverts H
-    | [H: Mu _ ::> _ |- _] => inverts H
+    | [H: Pair__sigma _ _ ::> _ |- _] => inverts H
+    | [H: Desc ::> _ |- _] => inverts H
+    | [H: Ind__desc ::> _ |- _] => inverts H
+    | [H: Sum__desc _ _ ::> _ |- _] => inverts H
+    | [H: Prd__desc _ _ ::> _ |- _] => inverts H
+    | [H: Unit__desc ::> _ |- _] => inverts H
+    | [H: Fix__desc _ ::> _ |- _] => inverts H
+    | [H: Mu _ _ ::> _ |- _] => inverts H
+    | [H: Wrap__mu _ ::> _ |- _] =>  inverts H
+    | [H: Inl__mu _ ::> _ |- _] => inverts H
+    | [H: Inr__mu _ ::> _ |- _] => inverts H
+    | [H: Pair__mu _ _ ::> _ |- _] => inverts H
+    | [H: Unit__mu ::> _ |- _] => inverts H
+    | [H: Fix__mu _ ::> _ |- _] => inverts H
   end.
 
 Notation spstep sigma tau := (forall v, sigma v ::> tau v).
@@ -166,12 +239,6 @@ Hint Rewrite sub_sig.
 Hint Resolve andb_true_intro.
 Hint Rewrite closed_sub_id using (auto; fail).
 
-Definition efunc_closed : forall D e, closed e -> closed (D_efunc D e).
-Proof. induction D; intros; simpl; rewrite asms; auto; simpl.
-  try_hyps; clear_funs; replace (D_efunc D2 e).[wk 1] with (D_efunc D2 e) by (autorewrite with core; auto).
-  eapply closed_lift; try eassumption; auto.
-Qed.
-
 Lemma sub_sig_scop : forall e sigma i j, sub_vars i j sigma -> closed_at j e -> sub_vars i.+1 j (e .: sigma).
 Proof. destruct v; simpl; auto. Qed.
 Hint Resolve sub_sig_scop.
@@ -179,25 +246,19 @@ Hint Resolve sub_sig_scop.
 Lemma sub_ids_scop : forall i, sub_vars i i ids. auto. Qed.
 Hint Resolve sub_ids_scop.
 
-Definition rall_scoped : forall D r e n, closed_at n.+1 r -> closed_at n e -> closed_at n (rall D r e).
-Proof. induction D; intros; simpl; rewrite asms; auto; simpl; auto;
-  apply sub_vars_scoped with (i := n.+1); auto; 
-  apply sub_sig_scop || apply sub_up_vars; auto.
-Qed.
-
-Hint Constructors par_step.
-
-Lemma rall_sub D : forall r e sigma, (rall D r e).[sigma] = rall D r.[up sigma] e.[sigma].
-Proof. induction D; intros; auto; simpl; rewrite asms; autosubst. Qed.
-Hint Rewrite rall_sub.   
-Hint Rewrite rall_sub : autosubst.
+(* Lemma rall_sub D : forall r e sigma, (rall D r e).[sigma] = rall D r.[up sigma] e.[sigma]. *)
+(* Proof. induction D; intros; auto; simpl; rewrite asms; autosubst. Qed. *)
+(* Hint Rewrite rall_sub.    *)
+(* Hint Rewrite rall_sub : autosubst. *)
 
 Hint Extern 1 (Free ?nm ::> ?e.[_]) => rewrite closed_sub_id; [constructor|eapply const_vals_closed]; eassumption.
 Hint Extern 1 (const_vals ?nm = Some ?e.[_]) => rewrite closed_sub_id; try eapply const_vals_closed; eassumption.
 Hint Resolve closed_sub_id.
+
+Optimize Heap.
 Lemma step_cong1 : forall e1 e2, e1 ::> e2 -> forall sigma, e1.[sigma] ::> e2.[sigma].
-Proof. induction 1; intros; simpl in *; subst; try solve[try econstructor; eauto; autosubst]. Qed.
-Local Hint Resolve step_cong1.
+Proof. induction 1; intros; simpl in *; subst; try solve[try econstructor step; eauto 1; autosubst]. Optimize Proof. Qed.
+Hint Resolve step_cong1.
 
 Lemma step_up : forall c1 c2, c1 .> c2 -> up c1 .> up c2.
 Proof. intros. destruct v; asimpl; auto. Qed.
@@ -212,13 +273,18 @@ Lemma step_cong2 : forall e c1 c2, c1 .> c2 -> e.[c1] ::> e.[c2].
 Proof. induction e; intros; simpl in *; try econstructor; eauto. Qed.
 
 Local Hint Resolve step_cong2.
+Optimize Heap.
 
 Lemma step_cong : forall e1 e2, e1 ::> e2 -> forall c1 c2, c1 .> c2 -> e1.[c1] ::> e2.[c2].
-Proof. induction 1; intros; simpl in *; subst; auto; econstructor;
-  try (eapply IHpar_step1 || eapply IHpar_step2); try (eapply step_upn || eapply step_up);
-  eassumption || autosubst.
+Proof. induction 1; intros; simpl in *; subst; auto;
+  econstructor step;
+  try (eapply IHpar_step1 || eapply IHpar_step2 || eapply IHpar_step3 || eapply IHpar_step4
+    || eapply IHpar_step5 || eapply IHpar_step6 || eapply IHpar_step7);
+  try (eapply step_upn || eapply step_up); eassumption || autosubst.
+  Optimize Proof.
 Qed.
 
+Optimize Heap.
 Hint Resolve step_cong.
 
 Lemma sub_cons : forall e e' sigma tau, e ::> e' -> sigma .> tau -> (e .: sigma) .> (e' .: tau). destruct v; simpl; auto. Qed.
@@ -228,13 +294,10 @@ Lemma up_ev : forall sigma tau, sigma .> tau -> up sigma .> up tau. destruct v; 
 
 Hint Resolve ids_ev up_ev sub_cons.
 
-Lemma rall_ev D : forall r r', r ::> r' -> forall e e', e ::>  e' -> rall D r e ::> rall D r' e'. induction D; simpl; auto. Qed.
-
-Hint Resolve rall_ev.
-
 Lemma rho_eval_from_to e e' : e ::> e' -> e' ::> rho e.
-Proof. induction 1; simpl; try (invert value steps || destruct match); subst; eauto 10; try solve by inversion.
-  inverts H; auto.
+Proof. induction 1; simpl; try (try (invert value step || destruct match); subst; eauto 10; solve by inversion).
+  destruct match; inverts H; auto.
+  Optimize Proof.
 Qed.
 
 Hint Resolve rho_eval_from_to.
@@ -244,81 +307,148 @@ Notation red := (clos_trans _ par_step).
 Infix "<:::>" := conv (at level 50).
 Infix ":::>" := red (at level 50).
 
-Instance red_refl : Reflexive red. auto. Qed.
+Tactic Notation "eauto" "tc" := eauto using clos_trans.
+Tactic Notation "eauto" "tc" integer(n) := eauto n using clos_trans.
+
+Lemma red_conv : forall e e', e :::> e' -> e <:::> e'. induction 1; eauto rst. Qed.
+Hint Resolve red_conv.
 
 Local Hint Resolve t_step rst_step rst_refl.
 Local Hint Resolve t_trans rst_trans rst_sym : slow.
 
-Lemma red_Pi_l : forall A B A', A :::> A' -> Pi A B :::> Pi A' B. induction 1; eauto. Qed.
-Lemma red_Pi_r : forall A B B', B :::> B' -> Pi A B :::> Pi A B'. induction 1; eauto. Qed.
+Hint Resolve rho_eval_to rho_eval_from_to.
+Lemma red_l_confl e1 e2 e3 : e1 ::> e2 -> e1 :::> e3 -> exists e4, e2 :::> e4 /\ e3 ::> e4.
+Proof. 
+  move=> He2 He3; move: e2 He2; induction He3; intros.
+  { eauto 7. }
+  { do 2 (try_hyps; intuition; destr_logic); clear_funs; eauto with slow. }
+Qed.
+  
+Lemma red_confl e1 e2 e3 : e1 :::> e2 -> e1 :::> e3 -> exists e4, e2 :::> e4 /\ e3 :::> e4.
+Proof.
+  move=>He2 He3; move: e3 He3; induction He2; intros.
+  { extend red_l_confl; try_hyps; destr_logic; eauto with slow. }
+  { do 2 (try_hyps; intuition; destr_logic); clear_funs; eauto with slow. }
+Qed.
+
+(* DO NOT hint resolve red_confl! slows conv_double_red a lot *)
+(* a nice corollary of confluence is equivalence of convertibility to convergence *)
+(* the convergence condition is sufficient for arbitrary relations, but only necessary for confluent ones *)
+Corollary conv_double_red : forall e1 e2, e1 <:::> e2 <-> (exists e3, e1 :::> e3 /\ e2 :::> e3).
+Proof.
+  split; move=>H; [|destr_logic; transitivity x; eauto with slow].
+  induction H; try solve[eauto].
+  - destr_logic; solve[eauto].
+  - destr_logic. extend red_confl.
+    try_hyps; clear_funs; destr_logic; solve[eauto with slow].
+Qed.
+
+(* Hint Resolve conv_double_red. *) (* not hinting because red_confl caused problems *)
+Hint Rewrite conv_double_red : unconv.
+
+Instance red_refl : Reflexive red. eauto tc. Qed.
+
+Lemma red_Pi_l : forall A B A', A :::> A' -> Pi A B :::> Pi A' B. induction 1; eauto tc. Qed.
+Lemma red_Pi_r : forall A B B', B :::> B' -> Pi A B :::> Pi A B'. induction 1; eauto tc. Qed.
 Local Hint Resolve red_Pi_l red_Pi_r.
 
-Lemma red_Pi_Pi A B A' B' : (A :::> A') -> (B :::> B') -> Pi A B :::> Pi A' B'. eauto. Qed.
+Lemma red_Pi_Pi A B A' B' : (A :::> A') -> (B :::> B') -> Pi A B :::> Pi A' B'. transitivity (Pi A B'); eauto tc. Qed.
 Hint Resolve red_Pi_Pi.
 
-Lemma red_Sigma_l : forall A B A', A :::> A' -> Sigma A B :::> Sigma A' B. induction 1; eauto. Qed.
-Lemma red_Sigma_r : forall A B B', B :::> B' -> Sigma A B :::> Sigma A B'. induction 1; eauto. Qed.
+Lemma red_Sigma_l : forall A B A', A :::> A' -> Sigma A B :::> Sigma A' B. induction 1; eauto tc. Qed.
+Lemma red_Sigma_r : forall A B B', B :::> B' -> Sigma A B :::> Sigma A B'. induction 1; eauto tc. Qed.
 Local Hint Resolve red_Sigma_l red_Sigma_r.
  
-Lemma red_Sigma_Sigma A B A' B' : (A :::> A') -> (B :::> B') -> Sigma A B :::> Sigma A' B'. eauto. Qed.
+Lemma red_Sigma_Sigma A B A' B' : (A :::> A') -> (B :::> B') -> Sigma A B :::> Sigma A' B'. transitivity (Sigma A B'); eauto tc. Qed.
 Hint Resolve red_Sigma_Sigma.
 
-Lemma red_Sum_l : forall A B A', A :::> A' -> Sum A B :::> Sum A' B. induction 1; eauto. Qed.
-Lemma red_Sum_r : forall A B B', B :::> B' -> Sum A B :::> Sum A B'. induction 1; eauto. Qed.
-Local Hint Resolve red_Sum_l red_Sum_r.
-
-Lemma red_Sum_Sum A B A' B' : (A :::> A') -> (B :::> B') -> Sum A B :::> Sum A' B'. eauto. Qed.
-Hint Resolve red_Sum_Sum.
-
-Lemma red_Lam_Lam : forall e e', e :::> e' -> Lam e :::> Lam e'. induction 1; eauto. Qed.
+Lemma red_Lam_Lam : forall e e', e :::> e' -> Lam e :::> Lam e'. induction 1; eauto tc. Qed.
 Hint Resolve red_Lam_Lam.
 
-Lemma red_Srec_l : forall r e r', r :::> r' -> S_rec r e :::> S_rec r' e. induction 1; auto; transitivity (S_rec y e); auto. Qed.
-Lemma red_Srec_r : forall r e e', e :::> e' -> S_rec r e :::> S_rec r e'. induction 1; auto; transitivity (S_rec r y); auto. Qed.
+Lemma red_Srec_l : forall r e r', r :::> r' -> Rec__sigma r e :::> Rec__sigma r' e. induction 1; auto; transitivity (Rec__sigma y e); auto. Qed.
+Lemma red_Srec_r : forall r e e', e :::> e' -> Rec__sigma r e :::> Rec__sigma r e'. induction 1; auto; transitivity (Rec__sigma r y); auto. Qed.
 Local Hint Resolve red_Srec_l red_Srec_r.
-Lemma red_Srec_Srec r e r' e' : r :::> r' -> e :::> e' -> S_rec r e :::> S_rec r' e'. transitivity (S_rec r' e); auto. Qed.
+Lemma red_Srec_Srec r e r' e' : r :::> r' -> e :::> e' -> Rec__sigma r e :::> Rec__sigma r' e'. transitivity (Rec__sigma r' e); auto. Qed.
 Hint Resolve red_Srec_Srec.
 
-Lemma red_Sum_inl_Sum_inl : forall e e', e :::> e' -> Sum_inl e :::> Sum_inl e'. induction 1; eauto. Qed.
-Lemma red_Sum_inr_Sum_inr : forall e e', e :::> e' -> Sum_inr e :::> Sum_inr e'. induction 1; eauto. Qed.
-Hint Resolve red_Sum_inl_Sum_inl red_Sum_inr_Sum_inr.
-
-Lemma red_App_l : forall A B A', A :::> A' -> App A B :::> App A' B. induction 1; eauto. Qed.
-Lemma red_App_r : forall A B B', B :::> B' -> App A B :::> App A B'. induction 1; eauto. Qed.
+Lemma red_App_l : forall A B A', A :::> A' -> App A B :::> App A' B. induction 1; eauto tc. Qed.
+Lemma red_App_r : forall A B B', B :::> B' -> App A B :::> App A B'. induction 1; eauto tc. Qed.
 Local Hint Resolve red_App_l red_App_r.
 
-Lemma red_App_App A B A' B' : (A :::> A') -> (B :::> B') -> App A B :::> App A' B'. eauto. Qed.
+Lemma red_App_App A B A' B' : (A :::> A') -> (B :::> B') -> App A B :::> App A' B'. transitivity (App A B'); eauto tc. Qed.
 Hint Resolve red_App_App.
 
-Lemma red_S_mk_l : forall A B A', A :::> A' -> S_mk A B :::> S_mk A' B. induction 1; eauto. Qed.
-Lemma red_S_mk_r : forall A B B', B :::> B' -> S_mk A B :::> S_mk A B'. induction 1; eauto. Qed.
-Local Hint Resolve red_S_mk_l red_S_mk_r.
+Lemma red_Pair_l : forall A B A', A :::> A' -> Pair__sigma A B :::> Pair__sigma A' B. induction 1; eauto tc. Qed.
+Lemma red_Pair_r : forall A B B', B :::> B' -> Pair__sigma A B :::> Pair__sigma A B'. induction 1; eauto tc. Qed.
+Local Hint Resolve red_Pair_l red_Pair_r.
 
-Lemma red_S_mk_S_mk a b a' b' : a :::> a' -> b :::> b' -> S_mk a b :::> S_mk a' b'. eauto. Qed.
-Hint Resolve red_S_mk_S_mk.
+Lemma red_Pair_Pair_sigma a b a' b' : a :::> a' -> b :::> b' -> Pair__sigma a b :::> Pair__sigma a' b'. transitivity (Pair__sigma a b'); eauto. Qed.
 
-Lemma red_Split_1 a b c a' : (a :::> a') -> Split a b c :::> Split a' b c. induction 1; auto; transitivity (Split y b c); auto. Qed.
-Lemma red_Split_2 a b c b' : (b :::> b') -> Split a b c :::> Split a b' c. induction 1; auto; transitivity (Split a y c); auto. Qed.
-Lemma red_Split_3 a b c c' : (c :::> c') -> Split a b c :::> Split a b c'. induction 1; auto; transitivity (Split a b y); auto. Qed.
-Local Hint Resolve red_Split_1 red_Split_2 red_Split_3.
+Hint Resolve red_Pair_Pair_sigma.
 
-Lemma red_Split_Split a b c a' b' c' : (a :::> a') -> (b :::> b') -> (c :::> c') -> Split a b c :::> Split a' b' c'.
-Proof. transitivity (Split a' b c); auto; transitivity (Split a' b' c); auto. Qed.
-Hint Resolve red_Split_Split.
+Lemma red_Path_l x y x' : x :::> x' -> Path x y :::> Path x' y. induction 1; eauto tc. Qed.
+Lemma red_Path_r x y y' : y :::> y' -> Path x y :::> Path x y'. induction 1; eauto tc. Qed.
+Local Hint Resolve red_Path_l red_Path_r.
 
-Lemma red_mu_l D : forall A B A', A :::> A' -> mu D A B :::> mu D A' B. induction 1; auto. transitivity (mu D y B); auto. Qed.
-Lemma red_mu_r D : forall A B B', B :::> B' -> mu D A B :::> mu D A B'. induction 1; auto; transitivity (mu D A y); auto. Qed.
-Local Hint Resolve red_mu_l red_mu_r.
+Lemma red_Path_Path x y x' y' : x :::> x' -> y :::> y' -> Path x y :::> Path x' y'. 
+Proof. transitivity (Path x' y); eauto. Qed.
+Hint Resolve red_Path_Path.
 
-Lemma red_mu_mu D A B A' B' : (A :::> A') -> (B :::> B') -> mu D A B :::> mu D A' B'. transitivity (mu D A' B); auto. Qed.
-Hint Resolve red_mu_mu.
+Lemma red_Refl_Refl x x' : x :::> x' -> Refl__path x :::> Refl__path x'. induction 1; eauto tc. Qed.
+Hint Resolve red_Refl_Refl.
+
+Lemma red_prec_prec_l c p c' : c :::> c' -> Rec__path c p :::> Rec__path c' p. induction 1; eauto tc. Qed.
+Lemma red_prec_prec_r c p p' : p :::> p' -> Rec__path c p :::> Rec__path c p'. induction 1; eauto tc. Qed.
+Local Hint Resolve red_prec_prec_l red_prec_prec_r.
+
+Lemma red_prec_prec c p c' p' : c :::> c' -> p :::> p' -> Rec__path c p :::> Rec__path c' p'.
+Proof. transitivity (Rec__path c' p); eauto. Qed.
+Hint Resolve red_prec_prec.
+
+Lemma red_Fix_Fix_desc F F' : F :::> F' -> Fix__desc F :::> Fix__desc F'. induction 1; eauto tc. Qed.
+Hint Resolve red_Fix_Fix_desc.
+
+Lemma red_Sum_l A B A' : A :::> A' -> Sum__desc A B :::> Sum__desc A' B. induction 1; eauto tc. Qed.
+Lemma red_Sum_r A B B' : B :::> B' -> Sum__desc A B :::> Sum__desc A B'. induction 1; eauto tc. Qed.
+Hint Resolve red_Sum_l red_Sum_r.
+
+Lemma red_Sum_Sum_desc A B A' B' : A :::> A' -> B :::> B' -> Sum__desc A B :::> Sum__desc A' B'. transitivity (Sum__desc A' B); eauto tc. Qed.
+Hint Resolve red_Sum_Sum_desc.
+
+Lemma red_Prd_l A B A' : A :::> A' -> Prd__desc A B :::> Prd__desc A' B. induction 1; eauto tc. Qed.
+Lemma red_Prd_r A B B' : B :::> B' -> Prd__desc A B :::> Prd__desc A B'. induction 1; eauto tc. Qed.
+Hint Resolve red_Prd_l red_Prd_r.
+
+Lemma red_Prd_Prd_desc A B A' B' : A :::> A' -> B :::> B' -> Prd__desc A B :::> Prd__desc A' B'. transitivity (Prd__desc A' B); eauto tc. Qed.
+Hint Resolve red_Prd_Prd_desc.
+
+Lemma red_descr_descr : forall i s p u f d i' s' p' u' f' d',
+                          i :::> i' -> s :::> s' -> p :::> p' -> u :::> u' -> f :::> f' -> d :::> d' ->
+                          Rec__desc i s p u f d :::> Rec__desc i' s' p' u' f' d'. Admitted. (* looks basically like the above *)
+Hint Resolve red_descr_descr.
+
+Lemma red_Mu_Mu : forall D1 D2 D1' D2', D1 :::> D1' -> D2 :::> D2' -> Mu D1 D2 :::> Mu D1' D2'. Admitted.
+Hint Resolve red_Mu_Mu.
+Lemma red_Inl_Inl : forall e e', e :::> e' -> Inl__mu e :::> Inl__mu e'. induction 1; eauto tc. Qed.
+Lemma red_Inr_Inr : forall e e', e :::> e' -> Inr__mu e :::> Inr__mu e'. induction 1; eauto tc. Qed.
+Hint Resolve red_Inl_Inl red_Inr_Inr.
+
+Lemma red_Fix_Fix_mu : forall f f', f :::> f' -> Fix__mu f :::> Fix__mu f'. induction 1; eauto tc. Qed.
+Lemma red_Wrap_Wrap_mu : forall m m', m :::> m' -> Wrap__mu m :::> Wrap__mu m'. induction 1; eauto tc. Qed.
+Lemma red_Pair_Pair_mu : forall a b a' b', a :::> a' -> b :::> b' -> Pair__mu a b :::> Pair__mu a' b'. Admitted.
+Hint Resolve red_Fix_Fix_mu red_Wrap_Wrap_mu red_Pair_Pair_mu.
+
+Lemma red_mur_mur : forall w il ir p u f m w' il' ir' p' u' f' m', 
+                      w :::> w' -> il :::> il' -> ir :::> ir' -> p :::> p' -> u :::> u' -> f :::> f' -> m :::> m' ->
+                      Rec__mu w il ir p u f m :::> Rec__mu w' il' ir' p' u' f' m'. Admitted.
+Hint Resolve red_mur_mur.
 
 Lemma red_Free nm e : Free nm :::> e <-> (e = Free nm) \/ (exists v, const_vals nm = Some v /\ v :::> e).
 Proof. remember (Free nm).
   split; induction 1; subst; auto.
-  - + inverts H; eauto.
-    + intuition; subst; destr_logic; eauto.
-  - destr_logic; eauto.
+  - + inverts H; eauto tc.
+    + intuition; subst; destr_logic; eauto tc.
+  - destr_logic; transitivity x; eauto.
 Qed.
 
 Lemma red_Bind v e : Bind v :::> e <-> e = Bind v. 
@@ -331,23 +461,23 @@ Proof. remember (Sort l).
   split; induction 1; subst; auto; inversion H; subst; intuition; subst; reflexivity.
 Qed.
 
-Lemma red_Unit e : Unit :::> e <-> e = Unit.
-Proof. remember Unit.
+Lemma red_Unit e : Unit__desc :::> e <-> e = Unit__desc.
+Proof. remember Unit__desc.
   split; induction 1; subst; auto; inversion H; subst; intuition; subst; reflexivity.
 Qed.
 
-Lemma red_unit e : unit :::> e <-> e = unit.
-Proof. remember unit.
+Lemma red_unit e : Unit__mu :::> e <-> e = Unit__mu.
+Proof. remember Unit__mu.
   split; induction 1; subst; auto; inversion H; subst; intuition; subst; reflexivity.
 Qed.
 
-Lemma red_Mu D e : Mu D :::> e <-> e = Mu D.
-Proof. remember (Mu D).
+Lemma red_Desc e : Desc :::> e <-> e = Desc.
+Proof. remember Desc.
   split; induction 1; subst; auto; inversion H; subst; intuition; subst; reflexivity.
 Qed.
 
-Hint Resolve red_Bind red_Sort red_Unit red_unit red_Mu.
-Hint Rewrite red_Bind red_Sort red_Unit red_unit red_Mu.
+Hint Resolve red_Bind red_Sort red_Unit red_unit red_Desc.
+Hint Rewrite red_Bind red_Sort red_Unit red_unit red_Desc.
 
 Lemma red_Pi A B e : Pi A B :::> e <-> exists A' B', (e = Pi A' B') /\ (A :::> A') /\ (B :::> B').
 Proof. split.
@@ -356,7 +486,8 @@ Proof. split.
     induction Hab; intros; subst; auto.
     { inversion H; subst; eauto 10. }
     { specialize (IHHab1 A B); intuition; destr_logic; subst.
-      specialize (IHHab2 x x0); intuition; destr_logic; subst. eauto 10. } }
+      specialize (IHHab2 x x0); intuition; destr_logic; subst.
+      repeat eexists; try reflexivity; eauto tc. } }
   { intros; destr_logic; subst; auto. }
 Qed.
 
@@ -367,34 +498,69 @@ Proof. split.
     induction Hab; intros; subst; auto.
     { inversion H; subst; eauto 10. }
     { specialize (IHHab1 A B); intuition; destr_logic; subst.
-      specialize (IHHab2 x x0); intuition; destr_logic; subst. eauto 10. } }
+      specialize (IHHab2 x x0); intuition; destr_logic; subst.
+      repeat eexists; try reflexivity; eauto tc. } }
   { intros; destr_logic; subst; auto. }
 Qed.
 
-Lemma red_S_mk A B e : S_mk A B :::> e <-> exists A' B', (e = S_mk A' B') /\ (A :::> A') /\ (B :::> B').
+Lemma red_Pair__sigma A B e : Pair__sigma A B :::> e <-> exists A' B', (e = Pair__sigma A' B') /\ (A :::> A') /\ (B :::> B').
 Proof. split.
-  { remember (S_mk A B) as ab. 
+  { remember (Pair__sigma A B) as ab. 
     move=>Hab. move:A B Heqab.
     induction Hab; intros; subst; auto.
     { inversion H; subst; eauto 10. }
     { specialize (IHHab1 A B); intuition; destr_logic; subst.
-      specialize (IHHab2 x x0); intuition; destr_logic; subst. eauto 10. } }
+      specialize (IHHab2 x x0); intuition; destr_logic; subst.
+      repeat eexists; try reflexivity; eauto tc. } }
   { intros; destr_logic; subst; auto. }
 Qed.
 
-Lemma red_Sum A B e : Sum A B :::> e <-> exists A' B', (e = Sum A' B') /\ (A :::> A') /\ (B :::> B').
+Lemma red_Prd__desc D1 D2 e : Prd__desc D1 D2 :::> e <-> exists D1' D2', (e = Prd__desc D1' D2') /\ (D1 :::> D1') /\ (D2 :::> D2').
 Proof. split.
-  { remember (Sum A B) as ab. 
-    move=>Hab. move:A B Heqab.
+  { remember (Prd__desc D1 D2) as m; move=>Hab. move:D1 D2 Heqm.
     induction Hab; intros; subst; auto.
     { inversion H; subst; eauto 10. }
-    { specialize (IHHab1 A B); intuition; destr_logic; subst.
-      specialize (IHHab2 x x0); intuition; destr_logic; subst. eauto 10. } }
+    { specialize (IHHab1 D1 D2); intuition; destr_logic; subst.
+      specialize (IHHab2 x x0); intuition; destr_logic; subst.
+      repeat eexists; try reflexivity; eauto tc. } }
   { intros; destr_logic; subst; auto. }
 Qed.
 
-Hint Resolve red_Pi red_Sigma red_S_mk red_Sum.
-Hint Rewrite red_Pi red_Sigma red_S_mk red_Sum.
+Lemma red_Sum__desc D1 D2 e : Sum__desc D1 D2 :::> e <-> exists D1' D2', (e = Sum__desc D1' D2') /\ (D1 :::> D1') /\ (D2 :::> D2').
+Proof. split.
+  { remember (Sum__desc D1 D2) as m; move=>Hab. move:D1 D2 Heqm.
+    induction Hab; intros; subst; auto.
+    { inversion H; subst; eauto 10. }
+    { specialize (IHHab1 D1 D2); intuition; destr_logic; subst.
+      specialize (IHHab2 x x0); intuition; destr_logic; subst.
+      repeat eexists; try reflexivity; eauto tc. } }
+  { intros; destr_logic; subst; auto. }
+Qed.
+
+Lemma red_Mu D1 D2 e : Mu D1 D2 :::> e <-> exists D1' D2', (e = Mu D1' D2') /\ (D1 :::> D1') /\ (D2 :::> D2').
+Proof. split.
+  { remember (Mu D1 D2) as m; move=>Hab. move:D1 D2 Heqm.
+    induction Hab; intros; subst; auto.
+    { inversion H; subst; eauto 10. }
+    { specialize (IHHab1 D1 D2); intuition; destr_logic; subst.
+      specialize (IHHab2 x x0); intuition; destr_logic; subst.
+      repeat eexists; try reflexivity; eauto tc. } }
+  { intros; destr_logic; subst; auto. }
+Qed.
+
+Lemma red_Pair__mu D1 D2 e : Pair__mu D1 D2 :::> e <-> exists D1' D2', (e = Pair__mu D1' D2') /\ (D1 :::> D1') /\ (D2 :::> D2').
+Proof. split.
+  { remember (Pair__mu D1 D2) as m; move=>Hab. move:D1 D2 Heqm.
+    induction Hab; intros; subst; auto.
+    { inversion H; subst; eauto 10. }
+    { specialize (IHHab1 D1 D2); intuition; destr_logic; subst.
+      specialize (IHHab2 x x0); intuition; destr_logic; subst.
+      repeat eexists; try reflexivity; eauto tc. } }
+  { intros; destr_logic; subst; auto. }
+Qed.
+
+Hint Resolve red_Pi red_Sigma red_Pair__sigma red_Prd__desc red_Sum__desc red_Mu red_Pair__mu.
+Hint Rewrite red_Pi red_Sigma red_Pair__sigma red_Prd__desc red_Sum__desc red_Mu red_Pair__mu.
 
 Lemma red_Lam b e : Lam b :::> e <-> exists b', (e = Lam b') /\ (b :::> b').
 Proof. split.
@@ -402,34 +568,64 @@ Proof. split.
     { inversion H; subst; eauto. }
     { specialize (IHHred1 b); intuition; destr_logic; subst.
       specialize (IHHred2 x); intuition; destr_logic; subst.
-      eauto. } }
+      eauto tc. } }
   { intros; destr_logic; subst; auto. }
 Qed.
 
-Lemma red_Sum_inl b e : Sum_inl b :::> e <-> exists b', (e = Sum_inl b') /\ (b :::> b').
+Lemma red_Fix__desc D e : Fix__desc D :::> e <-> exists D', (e = Fix__desc D') /\ (D :::> D').
 Proof. split.
-  { remember (Sum_inl b) as lb. move=>Hred; move: b Heqlb. induction Hred; intros; subst; eauto.
+  { remember (Fix__desc D) as lD. move=>Hred; move: D HeqlD. induction Hred; intros; subst; eauto.
+    { inversion H; subst; eauto. }
+    { specialize (IHHred1 D); intuition; destr_logic; subst.
+      specialize (IHHred2 x); intuition; destr_logic; subst.
+      eauto tc. } }
+  { intros; destr_logic; subst; auto. }
+Qed.
+
+Lemma red_Fix__mu c e : Fix__mu c :::> e <-> exists c', (e = Fix__mu c') /\ (c :::> c').
+Proof. split.
+  { remember (Fix__mu c) as lc. move=>Hred; move: c Heqlc. induction Hred; intros; subst; eauto.
+    { inversion H; subst; eauto. }
+    { specialize (IHHred1 c); intuition; destr_logic; subst.
+      specialize (IHHred2 x); intuition; destr_logic; subst.
+      eauto tc. } }
+  { intros; destr_logic; subst; auto. }
+Qed.
+
+Lemma red_Wrap__mu m e : Wrap__mu m :::> e <-> exists m', (e = Wrap__mu m') /\ (m :::> m').
+Proof. split.
+  { remember (Wrap__mu m) as lm. move=>Hred; move: m Heqlm. induction Hred; intros; subst; eauto.
+    { inversion H; subst; eauto. }
+    { specialize (IHHred1 m); intuition; destr_logic; subst.
+      specialize (IHHred2 x); intuition; destr_logic; subst.
+      eauto tc. } }
+  { intros; destr_logic; subst; auto. }
+Qed.
+
+Lemma red_Inl__mu b e : Inl__mu b :::> e <-> exists b', (e = Inl__mu b') /\ (b :::> b').
+Proof. split.
+  { remember (Inl__mu b) as lb. move=>Hred; move: b Heqlb. induction Hred; intros; subst; eauto.
     { inversion H; subst; eauto. }
     { specialize (IHHred1 b); intuition; destr_logic; subst.
       specialize (IHHred2 x); intuition; destr_logic; subst.
-      eauto. } }
+      eauto tc. } }
   { intros; destr_logic; subst; auto. }
 Qed.
 
-Lemma red_Sum_inr b e : Sum_inr b :::> e <-> exists b', (e = Sum_inr b') /\ (b :::> b').
+Lemma red_Inr__mu b e : Inr__mu b :::> e <-> exists b', (e = Inr__mu b') /\ (b :::> b').
 Proof. split.
-  { remember (Sum_inr b) as lb. move=>Hred; move: b Heqlb. induction Hred; intros; subst; eauto.
+  { remember (Inr__mu b) as lb. move=>Hred; move: b Heqlb. induction Hred; intros; subst; eauto.
     { inversion H; subst; eauto. }
     { specialize (IHHred1 _ erefl); destr_logic; subst.
       specialize (IHHred2 _ erefl); destr_logic; subst.
-      eauto. } }
+      eauto tc. } }
   { intros; destr_logic; subst; auto. }
 Qed.
 
-Hint Resolve red_Lam red_Sum_inl red_Sum_inr.
-Hint Rewrite red_Lam red_Sum_inl red_Sum_inr.
+Hint Resolve red_Lam red_Fix__desc red_Fix__mu red_Wrap__mu red_Inl__mu red_Inr__mu.
+Hint Rewrite red_Lam red_Fix__desc red_Fix__mu red_Wrap__mu red_Inl__mu red_Inr__mu.
 
-Lemma sred_cong1 : forall e e' sigma, e :::> e' -> e.[sigma] :::> e'.[sigma]. induction 1; eauto. Qed.
+Lemma sred_cong1 : forall e e' sigma, e :::> e' -> e.[sigma] :::> e'.[sigma]. induction 1; eauto tc. Qed.
 Local Hint Resolve sred_cong1.
 
 Notation sred sigma tau := (forall i : var, sigma i :::> tau i).
@@ -438,14 +634,17 @@ Infix "..>" := sred (at level 50).
 Lemma sred_ref : forall sigma, sigma ..> sigma. intros; eauto. Qed.
 Lemma sub_sred : forall sigma tau, sigma ..> tau -> forall e e', e :::> e' -> (e .: sigma) ..> (e' .: tau). intros; destruct i; simpl; auto. Qed.
 
-Lemma sred_trans : forall delta sigma tau, delta ..> sigma -> sigma ..> tau -> delta ..> tau. eauto. Qed.
+Lemma sred_trans : forall delta sigma tau, delta ..> sigma -> sigma ..> tau -> delta ..> tau. eauto tc. Qed.
 
 Lemma up_sred : forall sigma tau, sigma ..> tau -> up sigma ..> up tau. intros; destruct i; asimpl; auto. Qed.
 Hint Resolve up_sred sub_sred sred_ref.
 Lemma upn_sred n : forall sigma tau, sigma ..> tau -> upn n sigma ..> upn n tau. auto upn n. Qed.
 Hint Resolve upn_sred.
 
-Lemma sred_cong2 : forall e sigma tau, sigma ..> tau -> e.[sigma] :::> e.[tau]. induction e; intros; simpl; auto. Qed.
+(* CURRENT POINT *)
+Lemma sred_cong2 : forall e sigma tau, sigma ..> tau -> e.[sigma] :::> e.[tau]. induction e; intros; simpl; auto. 
+
+Qed.
 Local Hint Resolve sred_cong2.
 
 Lemma sred_cong : forall e e', e :::> e' -> forall sigma tau, sigma ..> tau -> e.[sigma] :::> e'.[tau]. intros. apply t_trans with (y := e.[tau]); auto. Qed.
@@ -458,189 +657,34 @@ Proof. split.
     move=>Hred; move: f a Heqfa; induction Hred; intros; subst.
     { inverts H; solve[left; eauto 7 | right; eauto 10]. }
     { specialize (IHHred1 _ _ erefl).
-      destr_logic; subst; [|right; eauto].
+      destr_logic; subst; [|right; eauto tc].
       specialize (IHHred2 _ _ erefl).
-      destr_logic; subst; [left|right]; eauto 7. } }
+      destr_logic; subst; [left|right]; eauto tc 7. } }
   { intros; destr_logic; subst; auto.
     eapply t_trans with (y := Lam _ :$: a);
       [|eapply t_trans with (y := _.[a/])]; eauto. }
 Qed.
 
-Lemma red_Srec r p e : S_rec r p :::> e <-> (exists r' p', e = S_rec r' p' /\ r :::> r' /\ p :::> p') \/
-                                          (exists a b, p :::> S_mk a b /\ r.[b,a/] :::> e).
+Lemma red_Srec r p e : Rec__sigma r p :::> e <-> (exists r' p', e = Rec__sigma r' p' /\ r :::> r' /\ p :::> p') \/
+                                          (exists a b, p :::> Pair__sigma a b /\ r.[b,a/] :::> e).
 Proof. split.
-  { remember (S_rec r p) as srp.
+  { remember (Rec__sigma r p) as srp.
     move=>Hred; move: r p Heqsrp; induction Hred; intros; subst.
     { inverts H; solve[left; eauto 7 | right; eauto 10]. }
     { specialize (IHHred1 _ _ erefl).
-      destr_logic; subst; [|right; eauto].
+      destr_logic; subst; [|right; eauto tc].
       specialize (IHHred2 _ _ erefl).
-      destr_logic; subst; [left|right]; eauto 7. } }
+      destr_logic; subst; [left|right]; eauto tc 7. } }
   { intros; destr_logic; subst; auto.
-    eapply t_trans with (y := S_rec r (S_mk _ _));
+    eapply t_trans with (y := Rec__sigma r (Pair__sigma _ _));
       [|eapply t_trans with (y := r.[_,_/])]; eauto. }
 Qed.
 
-Lemma red_Split a b c e : Split a b c :::> e <-> (exists a' b' c', e = Split a' b' c' /\ a :::> a' /\ b :::> b' /\ c :::> c')
-                                               \/ (exists a', c :::> Sum_inl a' /\ a.[a'/] :::> e)
-                                               \/ (exists b', c :::> Sum_inr b' /\ b.[b'/] :::> e).
-Proof. split.
-  { remember (Split a b c) as sabc.
-    move=>Hred; move: a b c Heqsabc; induction Hred; intros; subst.
-    { inversion H; subst; try solve[left;eauto 10|right;eauto 7]. }
-    { specialize (IHHred1 _ _ _ erefl).
-      destr_logic; subst; try solve[right;eauto].
-      specialize (IHHred2 _ _ _ erefl).
-      destr_logic; subst; try solve[left;eauto 10|right;eauto 7]. } }
-  { intros; destr_logic; subst; auto;
-    [eapply t_trans with (y := Split a b _); [|eapply t_trans with (y := a.[_/])]|
-     eapply t_trans with (y := Split a b _); [|eapply t_trans with (y := b.[_/])]]; eauto. }
-Qed.
-
-Lemma red_rall_l D r d r' : r :::> r' -> rall D r d :::> rall D r' d. induction 1; eauto. Qed.
-Lemma red_rall_r D r d d' : d :::> d' -> rall D r d :::> rall D r d'. induction 1; eauto. Qed.
-Local Hint Resolve red_rall_l red_rall_r.
-Lemma red_rall_rall D r d r' d' : r :::> r' -> d :::> d' -> rall D r d :::> rall D r' d'. eauto. Qed.
-Hint Resolve red_rall_rall.
-
-Lemma red_mu D r d e : mu D r d :::> e <-> (exists r' d', e = mu D r' d' /\ r :::> r' /\ d :::> d') 
-                                        \/ (r.[rall D (mu D r.[upn 2 (wk 1)] (Bind 0)) d, d/] :::> e).
-Proof. split.
-  { remember (mu D r d) as mdrd.
-    move=>Hred; move: r d Heqmdrd; induction Hred; intros; subst.
-    { inversion H; subst; try solve[left;eauto 7|right;eauto 10]. }
-    { specialize (IHHred1 _ _ erefl).
-      destr_logic; [subst|right;eauto].
-      specialize (IHHred2 _ _ erefl).
-      destr_logic; subst; [left;eauto 10|right].
-      eapply t_trans with (y := _.[_,_/]); try eassumption; apply sred_cong; auto. } }
-  { intros; destr_logic; subst; auto.
-    eapply t_trans with (y := _.[_,_/]); try eassumption; eauto. }
-Qed.
-
-Hint Rewrite red_Free red_App red_Srec red_Split red_mu : beta.
-
-Lemma red_conv : forall e e', e :::> e' -> e <:::> e'. induction 1; eauto with slow. Qed.
-Hint Resolve red_conv.
-
-Hint Resolve rho_eval_to rho_eval_from_to.
-Lemma red_l_confl e1 e2 e3 : e1 ::> e2 -> e1 :::> e3 -> exists e4, e2 :::> e4 /\ e3 ::> e4.
-Proof. 
-  move=> He2 He3; move: e2 He2; induction He3; intros.
-  { eauto 7. }
-  { do 2 (try_hyps; intuition; destr_logic); clear_funs; eauto. }
-Qed.
-  
-Lemma red_confl e1 e2 e3 : e1 :::> e2 -> e1 :::> e3 -> exists e4, e2 :::> e4 /\ e3 :::> e4.
-Proof.
-  move=>He2 He3; move: e3 He3; induction He2; intros.
-  { extend red_l_confl; try_hyps; destr_logic; eauto. }
-  { do 2 (try_hyps; intuition; destr_logic); clear_funs; eauto. }
-Qed.
-
-(* DO NOT hint resolve red_confl! slows conv_double_red a lot *)
-
-Lemma conv_double_red : forall e1 e2, e1 <:::> e2 <-> (exists e3, e1 :::> e3 /\ e2 :::> e3).
-Proof.
-  split; move=>H; [|destr_logic; eauto with slow].
-  induction H; try solve[eauto].
-  - destr_logic; solve[eauto].
-  - destr_logic. extend red_confl.
-    try_hyps; clear_funs; destr_logic; solve[eauto].
-Qed.
-
-(* Hint Resolve conv_double_red. *) (* not hinting because red_confl caused problems *)
-Hint Rewrite conv_double_red : unconv.
+Hint Rewrite red_Free red_App red_Srec : beta.
+(* let's see if we actually need the red_*rec lemmas - decent chance we will for some progress lemmas *)
 
 Notation sconv sigma tau := (forall i, sigma i <:::> tau i).
 Infix "<..>" := sconv (at level 20).
-
-Lemma conv_Bind_iff i j : Bind i <:::> Bind j <-> i = j. 
-Proof. autorewrite with unconv; split; intros; destr_logic; autorewrite with core in *; destr_logic; subst; congruence || eauto. Qed.
-
-Lemma conv_Sort_iff i j : Sort i <:::> Sort j <-> i = j. 
-Proof. autorewrite with unconv; split; intros; destr_logic; autorewrite with core in *; destr_logic; subst; congruence || eauto. Qed.
-
-Lemma conv_Mu_iff D1 D2 : Mu D1 <:::> Mu D2 <-> D1 = D2.
-Proof. autorewrite with unconv; split; intros; destr_logic; autorewrite with core in *; destr_logic; subst; congruence || eauto. Qed.
-
-Hint Rewrite conv_Bind_iff conv_Sort_iff conv_Mu_iff.
-
-Lemma conv_Lam_iff b1 b2 : Lam b1 <:::> Lam b2 <-> b1 <:::> b2.
-Proof. autorewrite with unconv; split; intros; destr_logic; autorewrite with core in *; destr_logic; eauto.
-  subst; inversion H0; subst; eauto.
-Qed.
-
-Lemma conv_Sum_inl_iff b1 b2 : Sum_inl b1 <:::> Sum_inl b2 <-> b1 <:::> b2.
-Proof. autorewrite with unconv; split; intros; destr_logic; autorewrite with core in *; destr_logic; eauto.
-  subst; inversion H0; subst; eauto.
-Qed.
-
-Lemma conv_Sum_inr_iff b1 b2 : Sum_inr b1 <:::> Sum_inr b2 <-> b1 <:::> b2.
-Proof. autorewrite with unconv; split; intros; destr_logic; autorewrite with core in *; destr_logic; eauto.
-  subst; inversion H0; subst; eauto.
-Qed.
-
-Hint Rewrite conv_Lam_iff conv_Sum_inl_iff conv_Sum_inr_iff.
-
-Lemma conv_Pi_iff A B A' B' : (Pi A B <:::> Pi A' B') <-> (A <:::> A' /\ B <:::> B').
-Proof. autorewrite with unconv; split; intros; destr_logic; autorewrite with core in *; destr_logic; eauto.
-  subst. inversion H0; subst. split; eauto.
-Qed.
-
-Lemma conv_Sigma_iff A B A' B' : (Sigma A B <:::> Sigma A' B') <-> (A <:::> A' /\ B <:::> B').
-Proof. autorewrite with unconv; split; intros; destr_logic; autorewrite with core in *; destr_logic; eauto.
-  subst. inversion H0; subst. split; eauto.
-Qed.
-
-Lemma conv_Sum_iff A B A' B' : (Sum A B <:::> Sum A' B') <-> (A <:::> A' /\ B <:::> B').
-Proof. autorewrite with unconv; split; intros; destr_logic; autorewrite with core in *; destr_logic; eauto.
-  subst. inversion H0; subst. split; eauto.
-Qed.
-
-Lemma conv_S_mk_iff A B A' B' : (S_mk A B <:::> S_mk A' B') <-> (A <:::> A' /\ B <:::> B').
-Proof. autorewrite with unconv; split; intros; destr_logic; autorewrite with core in *; destr_logic; eauto.
-  subst. inversion H0; subst. split; eauto.
-Qed.
-
-Hint Rewrite conv_Pi_iff conv_Sigma_iff conv_Sum_iff conv_S_mk_iff.
-
-Lemma conv_Pi_Pi A B A' B' : A <:::> A' -> B <:::> B' -> Pi A B <:::> Pi A' B'.
-Proof. autorewrite with core; auto. Qed.
-
-Lemma conv_Sigma_Sigma A B A' B' : A <:::> A' -> B <:::> B' -> Sigma A B <:::> Sigma A' B'.
-Proof. autorewrite with core; auto. Qed.
-
-Lemma conv_Sum_Sum A B A' B' : A <:::> A' -> B <:::> B' -> Sum A B <:::> Sum A' B'.
-Proof. autorewrite with core; auto. Qed.
-
-Lemma conv_S_mk_S_mk A B A' B' : A <:::> A' -> B <:::> B' -> S_mk A B <:::> S_mk A' B'.
-Proof. autorewrite with core; auto. Qed.
-
-Lemma conv_Lam_Lam : forall b1 b2, b1 <:::> b2 -> Lam b1 <:::> Lam b2. intros; autorewrite with core; auto. Qed.
-
-Hint Resolve conv_Pi_Pi conv_Sigma_Sigma conv_Sum_Sum conv_S_mk_S_mk conv_Lam_Lam.
-
-Lemma conv_Srec_Srec : forall r p r' p', r <:::> r' -> p <:::> p' -> S_rec r p <:::> S_rec r' p'.
-Proof. intros; autorewrite with unconv in *; destr_logic; eauto. Qed.
-
-Hint Resolve conv_Srec_Srec.
-
-Lemma conv_Sum_inl_Sum_inl : forall e e', e <:::> e' -> Sum_inl e <:::> Sum_inl e'. intros; autorewrite with core; auto. Qed.
-Lemma conv_Sum_inr_Sum_inr : forall e e', e <:::> e' -> Sum_inr e <:::> Sum_inr e'. intros; autorewrite with core; auto. Qed.
-Hint Resolve conv_Sum_inl_Sum_inl conv_Sum_inr_Sum_inr.
-
-Lemma conv_App_App f a f' a' : (f <:::> f') -> (a <:::> a') -> ((f :$: a) <:::> (f' :$: a')).
-Proof. autorewrite with unconv; intros; destr_logic; autorewrite with core in *; destr_logic; eauto. Qed.
-Hint Resolve conv_App_App.
-
-Lemma conv_Split_Split a b c a' b' c' : (a <:::> a') -> (b <:::> b') -> (c <:::> c') -> Split a b c <:::> Split a' b' c'.
-Proof. autorewrite with unconv; intros; destr_logic; autorewrite with core in *; destr_logic; eauto. Qed.
-Hint Resolve conv_Split_Split.
-
-Lemma conv_mu_mu D A B A' B' : (A <:::> A') -> (B <:::> B') -> mu D A B <:::> mu D A' B'.
-Proof. autorewrite with unconv; intros; destr_logic; autorewrite with core in *; destr_logic; eauto. Qed.
-Hint Resolve conv_mu_mu.
 
 Lemma sconv_cong1 sigma e1 e2 : e1 <:::> e2 -> e1.[sigma] <:::> e2.[sigma].
 Proof. autorewrite with unconv; intros; destr_logic; eauto. Qed.
@@ -653,44 +697,158 @@ Hint Resolve sconv_up.
 Lemma sconv_upn n sigma tau : sigma <..> tau -> upn n sigma <..> upn n tau. auto upn n. Qed.
 Hint Resolve sconv_upn.
 
+Optimize Heap.
 Lemma sconv_cong2 e : forall sigma tau, sigma <..> tau -> e.[sigma] <:::> e.[tau].
-Proof. induction e; simpl; auto 10. Qed.
+Proof. induction e; simpl; intros; auto;
+  repeat match goal with 
+           | [IH: forall sigma tau, sigma <..> tau -> _, H: ?sigma <..> ?tau |- _]
+             => pose proof (IH _ _ H); pose proof (IH _ _ (sconv_up _ _ H));
+               pose proof (IH _ _ (sconv_upn 2 _ _ H)); pose proof (IH _ _ (sconv_upn 4 _ _ H));
+               clear IH
+         end;
+  autorewrite with unconv in *; destr_logic; eauto.
+Qed.
 Hint Resolve sconv_cong2.
 
 Lemma sconv_cong e1 e2 sigma tau : e1 <:::> e2 -> sigma <..> tau -> e1.[sigma] <:::> e2.[tau]. intros; transitivity (e1.[tau]); auto. Qed.
 Hint Resolve sconv_cong.
 
-Definition subtyp A B := (A <:::> B \/ exists i j, A <:::> Sort i /\ B <:::> Sort j /\ i < j).
-Infix "::<<" := subtyp (at level 20).
+(* Lemma conv_Bind_iff i j : Bind i <:::> Bind j <-> i = j.  *)
+(* Proof. autorewrite with unconv; split; intros; destr_logic; autorewrite with core in *; destr_logic; subst; congruence || eauto. Qed. *)
 
-Lemma conv_sort_red e i : e <:::> Sort i <-> e :::> Sort i.
-Proof. split; [|auto]. autorewrite with unconv; intros; destr_logic; autorewrite with core in *; subst; auto. Qed.
-(* Hint Resolve conv_sort_red. *)
-Hint Rewrite conv_sort_red : unconv.
+(* Lemma conv_Sort_iff i j : Sort i <:::> Sort j <-> i = j.  *)
+(* Proof. autorewrite with unconv; split; intros; destr_logic; autorewrite with core in *; destr_logic; subst; congruence || eauto. Qed. *)
 
-Hint Resolve red_conv.
-Lemma conv_ext_l e1 e2 e3 : e1 <:::> e2 -> e2 :::> e3 -> e1 <:::> e3. eauto using clos_refl_sym_trans. Qed.
-Lemma conv_ext_r e1 e2 e3 : e1 :::> e2 -> e2 <:::> e3 -> e1 <:::> e3. eauto using clos_refl_sym_trans. Qed.
-Hint Resolve conv_ext_l conv_ext_r : slow.
+(* Lemma conv_Mu_iff D1 D2 : Mu D1 <:::> Mu D2 <-> D1 = D2. *)
+(* Proof. autorewrite with unconv; split; intros; destr_logic; autorewrite with core in *; destr_logic; subst; congruence || eauto. Qed. *)
 
-Instance subtyp_refl : Reflexive subtyp. unfold subtyp; auto. Qed.
+(* Hint Rewrite conv_Bind_iff conv_Sort_iff conv_Mu_iff. *)
 
-Hint Resolve sconv_cong1 sconv_cong2 sconv_cong.
+(* Lemma conv_Lam_iff b1 b2 : Lam b1 <:::> Lam b2 <-> b1 <:::> b2. *)
+(* Proof. autorewrite with unconv; split; intros; destr_logic; autorewrite with core in *; destr_logic; eauto. *)
+(*   subst; inversion H0; subst; eauto. *)
+(* Qed. *)
 
-Instance subtyp_trans : Transitive subtyp. 
-Proof. repeat destruct 1; destr_logic; autorewrite with core in *.
-  - left; eauto rst.
-  - right; eauto rst 7.
-  - assert (z <:::> Sort x1) by eauto using rst_trans,rst_sym.
-    right; eauto 7.
-  - assert (Sort x3 <:::> Sort x0) by eauto rst.
-    autorewrite with core in *; subst.
-    right; exists x2; exists x1; repeat split; [eauto rst|eauto rst|transitivity x0]; auto.
+(* Lemma conv_Inl__mu_iff b1 b2 : Inl__mu b1 <:::> Inl__mu b2 <-> b1 <:::> b2. *)
+(* Proof. autorewrite with unconv; split; intros; destr_logic; autorewrite with core in *; destr_logic; eauto. *)
+(*   subst; inversion H0; subst; eauto. *)
+(* Qed. *)
+
+(* Lemma conv_Inr__mu_iff b1 b2 : Inr__mu b1 <:::> Inr__mu b2 <-> b1 <:::> b2. *)
+(* Proof. autorewrite with unconv; split; intros; destr_logic; autorewrite with core in *; destr_logic; eauto. *)
+(*   subst; inversion H0; subst; eauto. *)
+(* Qed. *)
+
+(* Hint Rewrite conv_Lam_iff conv_Inl__mu_iff conv_Inr__mu_iff. *)
+
+(* Lemma conv_Pi_iff A B A' B' : (Pi A B <:::> Pi A' B') <-> (A <:::> A' /\ B <:::> B'). *)
+(* Proof. autorewrite with unconv; split; intros; destr_logic; autorewrite with core in *; destr_logic; eauto. *)
+(*   subst. inversion H0; subst. split; eauto. *)
+(* Qed. *)
+
+(* Lemma conv_Sigma_iff A B A' B' : (Sigma A B <:::> Sigma A' B') <-> (A <:::> A' /\ B <:::> B'). *)
+(* Proof. autorewrite with unconv; split; intros; destr_logic; autorewrite with core in *; destr_logic; eauto. *)
+(*   subst. inversion H0; subst. split; eauto. *)
+(* Qed. *)
+
+(* Lemma conv_Sum_iff A B A' B' : (Sum A B <:::> Sum A' B') <-> (A <:::> A' /\ B <:::> B'). *)
+(* Proof. autorewrite with unconv; split; intros; destr_logic; autorewrite with core in *; destr_logic; eauto. *)
+(*   subst. inversion H0; subst. split; eauto. *)
+(* Qed. *)
+
+(* Lemma conv_Pair__sigma_iff A B A' B' : (Pair__sigma A B <:::> Pair__sigma A' B') <-> (A <:::> A' /\ B <:::> B'). *)
+(* Proof. autorewrite with unconv; split; intros; destr_logic; autorewrite with core in *; destr_logic; eauto. *)
+(*   subst. inversion H0; subst. split; eauto. *)
+(* Qed. *)
+
+(* Hint Rewrite conv_Pi_iff conv_Sigma_iff conv_Sum_iff conv_Pair__sigma_iff. *)
+
+(* Lemma conv_Pi_Pi A B A' B' : A <:::> A' -> B <:::> B' -> Pi A B <:::> Pi A' B'. *)
+(* Proof. autorewrite with core; auto. Qed. *)
+
+(* Lemma conv_Sigma_Sigma A B A' B' : A <:::> A' -> B <:::> B' -> Sigma A B <:::> Sigma A' B'. *)
+(* Proof. autorewrite with core; auto. Qed. *)
+
+(* Lemma conv_Sum_Sum A B A' B' : A <:::> A' -> B <:::> B' -> Sum A B <:::> Sum A' B'. *)
+(* Proof. autorewrite with core; auto. Qed. *)
+
+(* Lemma conv_Pair__sigma_Pair__sigma A B A' B' : A <:::> A' -> B <:::> B' -> Pair__sigma A B <:::> Pair__sigma A' B'. *)
+(* Proof. autorewrite with core; auto. Qed. *)
+
+(* Lemma conv_Lam_Lam : forall b1 b2, b1 <:::> b2 -> Lam b1 <:::> Lam b2. intros; autorewrite with core; auto. Qed. *)
+
+(* Hint Resolve conv_Pi_Pi conv_Sigma_Sigma conv_Sum_Sum conv_Pair__sigma_Pair__sigma conv_Lam_Lam. *)
+
+(* Lemma conv_Srec_Srec : forall r p r' p', r <:::> r' -> p <:::> p' -> Rec__sigma r p <:::> Rec__sigma r' p'. *)
+(* Proof. intros; autorewrite with unconv in *; destr_logic; eauto. Qed. *)
+
+(* Hint Resolve conv_Srec_Srec. *)
+
+(* Lemma conv_Inl__mu_Inl__mu : forall e e', e <:::> e' -> Inl__mu e <:::> Inl__mu e'. intros; autorewrite with core; auto. Qed. *)
+(* Lemma conv_Inr__mu_Inr__mu : forall e e', e <:::> e' -> Inr__mu e <:::> Inr__mu e'. intros; autorewrite with core; auto. Qed. *)
+(* Hint Resolve conv_Inl__mu_Inl__mu conv_Inr__mu_Inr__mu. *)
+
+(* Lemma conv_App_App f a f' a' : (f <:::> f') -> (a <:::> a') -> ((f :$: a) <:::> (f' :$: a')). *)
+(* Proof. autorewrite with unconv; intros; destr_logic; autorewrite with core in *; destr_logic; eauto. Qed. *)
+(* Hint Resolve conv_App_App. *)
+
+(* Lemma conv_Split_Split a b c a' b' c' : (a <:::> a') -> (b <:::> b') -> (c <:::> c') -> Split a b c <:::> Split a' b' c'. *)
+(* Proof. autorewrite with unconv; intros; destr_logic; autorewrite with core in *; destr_logic; eauto. Qed. *)
+(* Hint Resolve conv_Split_Split. *)
+
+(* Lemma conv_mu_mu D A B A' B' : (A <:::> A') -> (B <:::> B') -> mu D A B <:::> mu D A' B'. *)
+(* Proof. autorewrite with unconv; intros; destr_logic; autorewrite with core in *; destr_logic; eauto. Qed. *)
+(* Hint Resolve conv_mu_mu. *)
+
+(* Definition subtyp A B := (A <:::> B \/ exists i j, A <:::> Sort i /\ B <:::> Sort j /\ i < j). *)
+(* Infix "::<<" := subtyp (at level 20). *)
+
+(* Lemma conv_sort_red e i : e <:::> Sort i <-> e :::> Sort i. *)
+(* Proof. split; [|auto]. autorewrite with unconv; intros; destr_logic; autorewrite with core in *; subst; auto. Qed. *)
+(* (* Hint Resolve conv_sort_red. *) *)
+(* Hint Rewrite conv_sort_red : unconv. *)
+
+(* Hint Resolve red_conv. *)
+(* Lemma conv_ext_l e1 e2 e3 : e1 <:::> e2 -> e2 :::> e3 -> e1 <:::> e3. eauto using clos_refl_sym_trans. Qed. *)
+(* Lemma conv_ext_r e1 e2 e3 : e1 :::> e2 -> e2 <:::> e3 -> e1 <:::> e3. eauto using clos_refl_sym_trans. Qed. *)
+(* Hint Resolve conv_ext_l conv_ext_r : slow. *)
+
+(* Instance subtyp_refl : Reflexive subtyp. unfold subtyp; auto. Qed. *)
+
+(* Hint Resolve sconv_cong1 sconv_cong2 sconv_cong. *)
+
+(* Instance subtyp_trans : Transitive subtyp.  *)
+(* Proof. repeat destruct 1; destr_logic; autorewrite with core in *. *)
+(*   - left; eauto rst. *)
+(*   - right; eauto rst 7. *)
+(*   - assert (z <:::> Sort x1) by eauto using rst_trans,rst_sym. *)
+(*     right; eauto 7. *)
+(*   - assert (Sort x3 <:::> Sort x0) by eauto rst. *)
+(*     autorewrite with core in *; subst. *)
+(*     right; exists x2; exists x1; repeat split; [eauto rst|eauto rst|transitivity x0]; auto. *)
+(* Qed. *)
+
+(* Lemma subtyp_cong1 A B sigma : subtyp A B -> subtyp A.[sigma] B.[sigma].  *)
+(* Proof. destruct 1; [left|right]; destr_logic; auto. *)
+(*   repeat eexists; *)
+(*   match goal with [|-context[Sort ?i]] => change (Sort i) with (Sort i).[sigma] | _ => eassumption end; *)
+(*   auto. *)
+(* Qed. *)
+
+Lemma closed_step e e' n : e ::> e' -> closed_at n e -> closed_at n e'.
+Proof.
+  move=> He'; move: n; induction He'; simpl in *; intros; subst;
+  autounfold in *; destr bands;
+  try solve[repeat (apply andb_true_intro; split); auto|
+  match goal with [H:  closed_at (?m.+1 + ?n) ?e = true
+                    ,IH: context[closed_at _ ?e = true -> closed_at _ ?e' = true]
+                    |-   context[?e'.[_]]] => 
+                    apply cons_scoped with (i := (m + n)) end;
+    [intro v; repeat match goal with [|-context[_ .: _]] => destruct v; simpl end; auto| |];
+    simpl; autounfold; autorewrite with core; firstorder].
+
+  - apply closed_lift with (i := 0); [|apply const_vals_closed with (nm := nm)]; auto.
+  - apply cons_scoped with (i := n); auto.
 Qed.
 
-Lemma subtyp_cong1 A B sigma : subtyp A B -> subtyp A.[sigma] B.[sigma]. 
-Proof. destruct 1; [left|right]; destr_logic; auto.
-  repeat eexists;
-  match goal with [|-context[Sort ?i]] => change (Sort i) with (Sort i).[sigma] | _ => eassumption end;
-  auto.
-Qed.
+Hint Resolve closed_step.
